port backtrack

Weidenbach_Book/IsaSAT_Backtrack.thy
@@ -712,8 +712,8 @@ definition propagate_bt_wl_D_heur
           lcount + 1, opts)
     })\<close>
 
-definition (in -) lit_of_hd_trail_st_heur :: \<open>twl_st_wl_heur \<Rightarrow> nat literal\<close> where
-  \<open>lit_of_hd_trail_st_heur S = lit_of_last_trail_pol (get_trail_wl_heur S)\<close>
+definition (in -) lit_of_hd_trail_st_heur :: \<open>twl_st_wl_heur \<Rightarrow> nat literal nres\<close> where
+  \<open>lit_of_hd_trail_st_heur S = do {ASSERT (fst (get_trail_wl_heur S) \<noteq> []); RETURN (lit_of_last_trail_pol (get_trail_wl_heur S))}\<close>
 
 definition remove_last
   :: \<open>nat literal \<Rightarrow> nat clause option \<Rightarrow> nat clause option nres\<close>
@@ -748,7 +748,7 @@ definition backtrack_wl_D_nlit_heur
     do {
       ASSERT(backtrack_wl_D_heur_inv S\<^sub>0);
       ASSERT(fst (get_trail_wl_heur S\<^sub>0) \<noteq> []);
-      let L = lit_of_hd_trail_st_heur S\<^sub>0;
+      L \<leftarrow> lit_of_hd_trail_st_heur S\<^sub>0;
       (S, n, C) \<leftarrow> extract_shorter_conflict_list_heur_st S\<^sub>0;
       ASSERT(get_clauses_wl_heur S = get_clauses_wl_heur S\<^sub>0);
       S \<leftarrow> find_decomp_wl_st_int n S;
@@ -853,14 +853,17 @@ proof -
     by (auto intro!: order_trans[of \<open>length (watched_by x1 x2)\<close> \<open>length (get_vdom x1a)\<close>])
 qed
 
-definition (in -) list_of_mset2
-  :: \<open>nat literal \<Rightarrow> nat literal \<Rightarrow> nat clause \<Rightarrow> nat clause_l nres\<close>
-where
-  \<open>list_of_mset2 L L' D =
-    SPEC (\<lambda>E. mset E = D \<and> E!0 = L \<and> E!1 = L' \<and> length E \<ge> 2)\<close>
-
 definition single_of_mset where
   \<open>single_of_mset D = SPEC(\<lambda>L. D = mset [L])\<close>
+
+(* TODO Move *)
+lemma length_list_ge2: \<open>length S \<ge> 2 \<longleftrightarrow> (\<exists>a b S'. S = [a, b] @ S')\<close>
+  apply (cases S)
+   apply (simp; fail)
+  apply (rename_tac a S')
+  apply (case_tac S')
+  by simp_all
+
 
 lemma backtrack_wl_D_nlit_backtrack_wl_D:
   \<open>(backtrack_wl_D_nlit_heur, backtrack_wl) \<in>
@@ -872,7 +875,7 @@ proof -
     do {
       ASSERT(backtrack_wl_D_heur_inv S\<^sub>0);
       ASSERT(fst (get_trail_wl_heur S\<^sub>0) \<noteq> []);
-      let L = lit_of_hd_trail_st_heur S\<^sub>0;
+      L \<leftarrow> lit_of_hd_trail_st_heur S\<^sub>0;
       (S, n, C) \<leftarrow> extract_shorter_conflict_list_heur_st S\<^sub>0;
       ASSERT(get_clauses_wl_heur S = get_clauses_wl_heur S\<^sub>0);
       S \<leftarrow> find_decomp_wl_st_int n S;
@@ -957,17 +960,17 @@ proof -
       corr: \<open>correct_watching S\<close> and
       T_U: \<open>(T, U) \<in> twl_st_l None\<close> and
       trail_nempty: \<open>get_trail_l T \<noteq> []\<close> and
-      nss: \<open>\<forall>S'. \<not> cdcl\<^sub>W_restart_mset.skip (state\<^sub>W_of U) S'\<close> and
-      nsr: \<open>\<forall>S'. \<not> cdcl\<^sub>W_restart_mset.resolve (state\<^sub>W_of U) S'\<close> and
       not_none: \<open>get_conflict_l T \<noteq> None\<close> and
       struct_invs: \<open>twl_struct_invs U\<close> and
       stgy_invs: \<open>twl_stgy_invs U\<close> and
       list_invs: \<open>twl_list_invs T\<close> and
-      not_empty: \<open>get_conflict_l T \<noteq> Some {#}\<close>
-      using inv unfolding backtrack_wl_inv_def backtrack_wl_inv_def backtrack_l_inv_def
+      not_empty: \<open>get_conflict_l T \<noteq> Some {#}\<close> and
+      uL_D: \<open>- lit_of (hd (get_trail_wl S)) \<in># the (get_conflict_wl S)\<close> and
+      nss: \<open>no_step cdcl\<^sub>W_restart_mset.skip (state\<^sub>W_of U)\<close> and
+      nsr: \<open>no_step cdcl\<^sub>W_restart_mset.resolve (state\<^sub>W_of U)\<close>
+      using inv unfolding backtrack_wl_inv_def backtrack_wl_inv_def backtrack_l_inv_def backtrack_inv_def
       apply -
-      apply normalize_goal+
-      by blast
+      apply normalize_goal+ by simp
     have D_none: \<open>D \<noteq> None\<close>
       using S_T not_none by (auto simp: S)
     have b: \<open>\<not>b\<close>
@@ -976,10 +979,6 @@ proof -
       \<open>cdcl\<^sub>W_restart_mset.cdcl\<^sub>W_all_struct_inv (state\<^sub>W_of U)\<close>
       using struct_invs
       by (auto simp: twl_struct_invs_def)
-    then have uL_D: \<open>- lit_of (hd (get_trail_wl S)) \<in># the (get_conflict_wl S)\<close>
-      using cdcl\<^sub>W_restart_mset.no_step_skip_hd_in_conflicting[of
-          \<open>state\<^sub>W_of U\<close>] nss not_none not_empty stgy_invs trail_nempty S_T T_U
-      by (auto simp: twl_st_wl twl_st twl_stgy_invs_def)
     have
       \<open>cdcl\<^sub>W_restart_mset.no_strange_atm (state\<^sub>W_of U)\<close> and
       lev_inv: \<open>cdcl\<^sub>W_restart_mset.cdcl\<^sub>W_M_level_inv (state\<^sub>W_of U)\<close> and
@@ -1449,7 +1448,7 @@ proof -
           get_clauses_wl_heur U = get_clauses_wl_heur S) \<and>
 	  (get_trail_wl U'', get_vmtf_heur U) \<in> (Id \<times>\<^sub>f (Id \<times>\<^sub>f (distinct_atoms_rel (all_atms_st T'))\<inverse>)) ``
 	    (Collect (find_decomp_w_ns_prop (all_atms_st T') (get_trail_wl T') n (get_vmtf_heur T)))}
-          (find_decomp_wl (lit_of (hd (get_trail_wl S'))) T')\<close>
+          (find_decomp_wl LK' T')\<close>
     (is \<open>_ \<le>  \<Down> ?find_decomp _\<close>)
     if
       \<open>(S, S') \<in> ?R\<close> and
@@ -1457,8 +1456,9 @@ proof -
       \<open>backtrack_wl_D_heur_inv S\<close> and
       TT': \<open>(TnC, T') \<in> ?shorter S' S\<close> and
       [simp]: \<open>nC = (n, C)\<close> and
-      [simp]: \<open>TnC = (T, nC)\<close>
-    for S S' TnC T' T nC n C
+      [simp]: \<open>TnC = (T, nC)\<close> and
+       KK': \<open>(LK, LK') \<in> {(L, L'). L = L' \<and> L = lit_of (hd (get_trail_wl S'))}\<close>
+    for S S' TnC T' T nC n C LK LK'
   proof -
     obtain M N D NE UE Q W where
       T': \<open>T' = (M, N, D, NE, UE, Q, W)\<close>
@@ -1478,6 +1478,11 @@ proof -
       vm0: \<open>vm0 \<in> vmtf (all_atms_st T') M\<close>
       using vm unfolding isa_vmtf_def by (cases vm) auto
 
+    have [simp]:
+       \<open>LK' = lit_of (hd (get_trail_wl T'))\<close>
+       \<open>LK = LK'\<close>
+       using KK' TT' by (auto simp: equality_except_conflict_wl_get_trail_wl)
+
     have n: \<open>n = get_maximum_level M (remove1_mset (- lit_of (hd M)) (mset C))\<close> and
       eq: \<open>equality_except_conflict_wl T' S'\<close> and
       \<open>the D = mset C\<close> \<open>D \<noteq> None\<close> and
@@ -1486,7 +1491,7 @@ proof -
       bounded: \<open>isasat_input_bounded (all_atms_st T')\<close> and
       T_T': \<open>(T, del_conflict_wl T') \<in> twl_st_heur_bt\<close> and
       n2: \<open>n = get_maximum_level M (remove1_mset (- lit_of (hd M)) (the D))\<close>
-      using TT' by (auto simp: T T' twl_st_heur_bt_def del_conflict_wl_def simp flip: all_atms_def
+      using TT' KK' by (auto simp: T T' twl_st_heur_bt_def del_conflict_wl_def simp flip: all_atms_def
           simp del: isasat_input_bounded_def)
     have [simp]: \<open>get_trail_wl S' = M\<close>
       using eq \<open>the D = mset C\<close> \<open>D \<noteq> None\<close> by (cases S'; auto simp: T')
@@ -1526,26 +1531,26 @@ proof -
           intro!: RETURN_RES_refine
           intro: isa_vmtfI)
       apply (rule_tac x=an in exI)
-      apply (auto dest: no_dup_appendD intro: isa_vmtfI)
-      apply (auto simp: Image_iff)
+      apply (auto dest: no_dup_appendD intro: isa_vmtfI simp: T')
+      apply (auto simp: Image_iff T')
       done
   qed
 
   have fst_find_lit_of_max_level_wl: \<open>RETURN (C ! 1)
       \<le> \<Down> Id
-          (find_lit_of_max_level_wl U'
-            (lit_of (hd (get_trail_wl S'))))\<close>
+          (find_lit_of_max_level_wl U' LK')\<close>
     if
       \<open>(S, S') \<in> ?R\<close> and
-      \<open>backtrack_wl_D_inv S'\<close> and
+      \<open>backtrack_wl_inv S'\<close> and
       \<open>backtrack_wl_D_heur_inv S\<close> and
-      \<open>(TnC, T') \<in> ?shorter S' S\<close> and
+      TT': \<open>(TnC, T') \<in> ?shorter S' S\<close> and
       [simp]: \<open>nC = (n, C)\<close> and
       [simp]: \<open>TnC = (T, nC)\<close> and
       find_decomp: \<open>(U, U') \<in> ?find_decomp S T' n\<close> and
       size_C: \<open>1 < length C\<close> and
-      size_conflict_U': \<open>1 < size (the (get_conflict_wl U'))\<close>
-    for S S' TnC T' T nC n C U U'
+      size_conflict_U': \<open>1 < size (the (get_conflict_wl U'))\<close> and
+       KK': \<open>(LK, LK') \<in> {(L, L'). L = L' \<and> L = lit_of (hd (get_trail_wl S'))}\<close>
+    for S S' TnC T' T nC n C U U' LK LK'
   proof -
     obtain M N NE UE Q W where
       T': \<open>T' = (M, N, Some (mset C), NE, UE, Q, W)\<close> and
@@ -1561,6 +1566,11 @@ proof -
       using \<open>(TnC, T') \<in> ?shorter S' S\<close> \<open>1 < length C\<close> find_decomp
       by (cases U'; cases S')
         (auto simp: find_lit_of_max_level_wl_def T')
+
+    have [simp]:
+       \<open>LK' = lit_of (hd (get_trail_wl T'))\<close>
+       \<open>LK = LK'\<close>
+       using KK' TT' by (auto simp: equality_except_conflict_wl_get_trail_wl)
 
     have n_d: \<open>no_dup (get_trail_wl S')\<close>
       using \<open>(S, S') \<in> ?R\<close>
@@ -1597,11 +1607,12 @@ proof -
       using \<open>(TnC, T') \<in> ?shorter S' S\<close> \<open>1 < length C\<close> hd_conv_nth[OF \<open>C \<noteq> []\<close>, symmetric]
       by (auto simp: find_lit_of_max_level_wl_def U' highest_lit_def T')
   qed
-  have propagate_bt_wl_D_heur: \<open>propagate_bt_wl_D_heur (lit_of_hd_trail_st_heur S) C U
-      \<le> \<Down> ?S (propagate_bt_wl_D (lit_of (hd (get_trail_wl S'))) L' U')\<close>
+
+  have propagate_bt_wl_D_heur: \<open>propagate_bt_wl_D_heur LK C U
+      \<le> \<Down> ?S (propagate_bt_wl LK' L' U')\<close>
     if
       SS': \<open>(S, S') \<in> ?R\<close> and
-      \<open>backtrack_wl_D_inv S'\<close> and
+      \<open>backtrack_wl_inv S'\<close> and
       \<open>backtrack_wl_D_heur_inv S\<close> and
       \<open>(TnC, T') \<in> ?shorter S' S\<close> and
       [simp]: \<open>nC = (n, C)\<close> and
@@ -1609,9 +1620,11 @@ proof -
       find_decomp: \<open>(U, U') \<in> ?find_decomp S T' n\<close> and
       le_C: \<open>1 < length C\<close> and
       \<open>1 < size (the (get_conflict_wl U'))\<close> and
-      C_L': \<open>(C ! 1, L') \<in> nat_lit_lit_rel\<close>
-    for S S' TnC T' T nC n C U U' L'
+      C_L': \<open>(C ! 1, L') \<in> nat_lit_lit_rel\<close> and
+      KK': \<open>(LK, LK') \<in> {(L, L'). L = L' \<and> L = lit_of (hd (get_trail_wl S'))}\<close>
+    for S S' TnC T' T nC n C U U' L' LK LK'
   proof -
+
     have
       TT': \<open>(T, del_conflict_wl T') \<in> twl_st_heur_bt\<close> and
       n: \<open>n = get_maximum_level (get_trail_wl T')
@@ -1672,6 +1685,11 @@ proof -
         U: \<open>U = (M1', arena, D', Q', W', vm', \<phi>, clvls, cach, lbd, outl, stats, (fema, sema, ccount),
            vdom, avdom, lcount, opts, [])\<close>
       using UU' find_decomp by (cases U) (auto simp: U' T' twl_st_heur_bt_def all_atms_def[symmetric])
+
+    have [simp]:
+       \<open>LK' = lit_of (hd M)\<close>
+       \<open>LK = LK'\<close>
+       using KK' SS' by (auto simp: equality_except_conflict_wl_get_trail_wl S')
     have
       M1'_M1: \<open>(M1', M1) \<in> trail_pol (all_atms_st U')\<close> and
       W'W: \<open>(W', W) \<in> \<langle>Id\<rangle>map_fun_rel (D\<^sub>0 (all_atms_st U'))\<close> and
@@ -1756,12 +1774,29 @@ proof -
       })\<close>
       unfolding propagate_bt_wl_D_heur_def Let_def
       by auto
+    have find_new_alt: \<open>SPEC
+                 (\<lambda>(N', i). N' = fmupd i (D'', False) N \<and> 0 < i \<and>
+                      i \<notin># dom_m N \<and>
+                      (\<forall>L\<in>#all_lits_of_mm (mset `# ran_mf N + (NE + UE)).
+                          i \<notin> fst ` set (W L))) = do {
+
+          i \<leftarrow> SPEC
+                 (\<lambda>i. 0 < i \<and>
+                      i \<notin># dom_m N \<and>
+                      (\<forall>L\<in>#all_lits_of_mm (mset `# ran_mf N + (NE + UE)).
+                          i \<notin> fst ` set (W L)));
+         N' \<leftarrow> RETURN (fmupd i (D'', False) N);
+         RETURN (N', i)
+      }\<close> for D''
+      by (auto simp: RETURN_def RES_RES_RETURN_RES2
+       RES_RES_RETURN_RES)
     have propagate_bt_wl_D_alt_def:
-      \<open>propagate_bt_wl (lit_of (hd (get_trail_wl S'))) L' U' = do {
+      \<open>propagate_bt_wl LK' L' U' = do {
+            ASSERT (propagate_bt_wl_pre LK' L' (M1, N, Some (mset C), NE, UE, Q, W));
             _ \<leftarrow> RETURN (); \<^cancel>\<open>phase saving\<close>
             _ \<leftarrow> RETURN (); \<^cancel>\<open>LBD\<close>
             D'' \<leftarrow>
-              list_of_mset2 (- lit_of (hd (get_trail_wl S'))) L'
+              list_of_mset2 (- LK') L'
                (the (Some (mset C)));
             (N, i) \<leftarrow> SPEC
                  (\<lambda>(N', i). N' = fmupd i (D'', False) N \<and> 0 < i \<and>
@@ -1770,21 +1805,22 @@ proof -
                           i \<notin> fst ` set (W L)));
             _ \<leftarrow> RETURN (); \<^cancel>\<open>lbd empty\<close>
             _ \<leftarrow> RETURN (); \<^cancel>\<open>lbd empty\<close>
-	     M2 \<leftarrow> RETURN (Propagated (- lit_of (hd (get_trail_wl S'))) i # M1);
+	     M2 \<leftarrow> cons_trail_propagate_l (- LK') i M1;
             _ \<leftarrow> RETURN (); \<^cancel>\<open>vmtf_flush\<close>
             RETURN
               (M2,
-                N, None, NE, UE, unmark (hd (get_trail_wl S')),
-                W(- lit_of (hd (get_trail_wl S')) :=
-                   W (- lit_of (hd (get_trail_wl S'))) @ [(i, L', length D'' = 2)],
-                  L' := W L' @ [(i, - lit_of (hd (get_trail_wl S')), length D'' = 2)]))
+                N, None, NE, UE, {#LK'#},
+                W(- LK' := W (- LK') @ [(i, L', length D'' = 2)],
+                  L' := W L' @ [(i, - LK', length D'' = 2)]))
           }\<close>
-      unfolding propagate_bt_wl_def Let_def
+      unfolding propagate_bt_wl_def Let_def find_new_alt nres_monad3
         U U' H get_fresh_index_wl_def prod.case
         propagate_bt_wl_def Let_def rescore_clause_def
       by (auto simp: U' RES_RES2_RETURN_RES RES_RETURN_RES \<phi> uminus_\<A>\<^sub>i\<^sub>n_iff
-          uncurry_def RES_RES_RETURN_RES
-          get_fresh_index_def RES_RETURN_RES2 RES_RES_RETURN_RES2 list_of_mset2_def)
+          uncurry_def RES_RES_RETURN_RES length_list_ge2
+          get_fresh_index_def RES_RETURN_RES2 RES_RES_RETURN_RES2 list_of_mset2_def
+          intro!: bind_cong[OF refl])
+
     have [refine0]: \<open>SPEC (\<lambda>(vm', \<phi>'). vm' \<in> vmtf \<A> M1 \<and> phase_saving \<A> \<phi>')
        \<le> \<Down>{((vm', \<phi>'), ()). vm' \<in> vmtf \<A> M1 \<and> phase_saving \<A> \<phi>'} (RETURN ())\<close> for \<A>
       by (auto intro!: RES_refine simp: RETURN_def)
@@ -1808,48 +1844,49 @@ proof -
       subgoal using vm M1'_M1 by auto
       subgoal by (auto simp: rescore_clause_def conc_fun_RES intro!: isa_vmtfI)
       done
-(*
-    have [refine0]: \<open>isa_vmtf_flush_int (cons_trail_Propagated_tr L i M1') vm \<le>
-         SPEC(\<lambda>c. (c, ()) \<in> {(vm', _). vm' \<in> isa_vmtf (all_atms_st U') (Propagated L i # M1)})\<close>
+
+    have [refine0]: \<open>isa_vmtf_flush_int Ma vm \<le>
+         SPEC(\<lambda>c. (c, ()) \<in> {(vm', _). vm' \<in> isa_vmtf (all_atms_st U') M2})\<close>
       if vm: \<open>vm \<in> isa_vmtf (all_atms_st U') M1\<close> and
-      	L: \<open>L \<in># \<L>\<^sub>a\<^sub>l\<^sub>l (all_atms_st U')\<close> and
-      	undef: \<open>undefined_lit M1 L\<close> and
-      	i: \<open>i \<noteq> DECISION_REASON\<close>
-      for vm i L
+       Ma: \<open>(Ma, M2)
+       \<in> {(M0, M0'').
+         (M0, M0'') \<in> trail_pol (all_atms_st U') \<and>
+         M0'' = Propagated (- L) i # M1 \<and>
+         no_dup M0''}\<close>
+      for vm i L Ma M2
     proof -
       let ?M1' = \<open>cons_trail_Propagated_tr L i M1'\<close>
-      let ?M1 = \<open>cons_trail_Propagated L i M1\<close>
+      let ?M1 = \<open>Propagated (-L) i # M1\<close>
 
-      have M1'_M1: \<open>(?M1', ?M1) \<in> trail_pol (all_atms_st U')\<close>
-        unfolding cons_trail_Propagated_def
-        by (rule cons_trail_Propagated_tr2[OF M1'_M1 L undef i])
+      have M1'_M1: \<open>(Ma, M2) \<in> trail_pol (all_atms_st U')\<close>
+        using Ma by auto
 
       have vm: \<open>vm \<in> isa_vmtf (all_atms_st U') ?M1\<close>
-        using vm by (auto simp: isa_vmtf_def cons_trail_Propagated_def dest: vmtf_consD)
+        using vm by (auto simp: isa_vmtf_def dest: vmtf_consD)
       obtain vm0 where
         vm: \<open>(vm, vm0) \<in> Id \<times>\<^sub>r distinct_atoms_rel (all_atms_st U')\<close> and
         vm0: \<open>vm0 \<in> vmtf (all_atms_st U') ?M1\<close>
         using vm unfolding isa_vmtf_def by (cases vm) auto
       show ?thesis
       	apply (rule order.trans)
-      	 apply (rule isa_vmtf_flush_int[THEN fref_to_Down_curry, of _ _ ?M1])
-      	  apply ((solves \<open>use M1'_M1 in auto\<close>)+)[2]
+      	 apply (rule isa_vmtf_flush_int[THEN fref_to_Down_curry, of _ _ ?M1 vm])
+      	  apply ((solves \<open>use M1'_M1 Ma in auto\<close>)+)[2]
       	apply (subst Down_id_eq)
       	apply (rule order.trans)
       	 apply (rule vmtf_change_to_remove_order'[THEN fref_to_Down_curry, of \<open>all_atms_st U'\<close> ?M1 vm0 ?M1 vm])
       	subgoal using vm0 bounded nempty by auto
       	subgoal using vm by auto
-      	subgoal by (auto simp: vmtf_flush_def conc_fun_RES RETURN_def intro: isa_vmtfI)
+      	subgoal using Ma by (auto simp: vmtf_flush_def conc_fun_RES RETURN_def intro: isa_vmtfI)
       	done
     qed
-*)
+
     have [refine0]: \<open>(isa_length_trail M1', ()) \<in> {(j, _). j = length M1}\<close>
       by (subst isa_length_trail_length_u[THEN fref_to_Down_unRET_Id, OF _ M1'_M1]) auto
     have [refine0]: \<open>get_LBD lbd \<le> \<Down> {(_, _). True}(RETURN ())\<close>
       unfolding get_LBD_def by (auto intro!: RES_refine simp: RETURN_def)
     have [refine0]: \<open>RETURN C
        \<le> \<Down> Id
-          (list_of_mset2 (- lit_of (hd (get_trail_wl S'))) L'
+          (list_of_mset2 (- LK') L'
             (the (Some (mset C))))\<close>
       using that
       by (auto simp: list_of_mset2_def S')
@@ -1893,14 +1930,7 @@ proof -
     have [refine0]:
       \<open>lbd_empty lbd \<le> SPEC (\<lambda>c. (c, ()) \<in> {(c, _). c = replicate (length lbd) False})\<close>
       by (auto simp: lbd_empty_def)
-    have [of _ _ \<open>all_atms_st U'\<close>, refine0]: \<open>undefined_lit M L \<and> L \<in># \<L>\<^sub>a\<^sub>l\<^sub>l \<A> \<and> C \<noteq> DECISION_REASON \<Longrightarrow>
-       (((L', C'), M'), (L, C), M) \<in> nat_lit_lit_rel \<times>\<^sub>f nat_rel \<times>\<^sub>f trail_pol \<A> \<Longrightarrow>
-       cons_trail_Propagated_tr L' C' M'
-         \<le> \<Down> {(M0, M0''). (M0, M0'') \<in> trail_pol \<A> \<and> M0'' = Propagated L C' # M}
-	     (RETURN (Propagated L C # M))\<close> for C C' :: nat and L and L' and M M' \<A>
-      using cons_trail_Propagated_tr[of \<A>, THEN fref_to_Down_curry2, of L C M L' C' M']
-      apply (auto simp: cons_trail_Propagated_tr_def)
-find_theorems cons_trail_Propagated_tr
+
     have \<open>literals_are_in_\<L>\<^sub>i\<^sub>n (all_atms_st S') (mset C)\<close>
       using incl list_confl_S' literals_are_in_\<L>\<^sub>i\<^sub>n_mono by blast
     then have C_Suc1_in: \<open>C ! Suc 0 \<in># \<L>\<^sub>a\<^sub>l\<^sub>l (all_atms_st S')\<close>
@@ -1918,10 +1948,6 @@ find_theorems cons_trail_Propagated_tr
     have tr_SS': \<open>(get_trail_wl_heur S, M) \<in> trail_pol (all_atms_st S')\<close>
       using \<open>(S, S') \<in> ?R\<close> unfolding twl_st_heur_conflict_ana_def
       by (auto simp: all_atms_def S')
-    have hd_tr_S_M: \<open>lit_of_hd_trail_st_heur S = lit_of_hd_trail M\<close>
-      unfolding lit_of_hd_trail_def lit_of_hd_trail_st_heur_def
-      by (subst lit_of_last_trail_pol_lit_of_last_trail[THEN fref_to_Down_unRET_Id, OF _ tr_SS'])
-        (use tr_nempty in \<open>auto simp: lit_of_hd_trail_def T'\<close>)
     have All_atms_rew: \<open>set_mset (all_atms (fmupd x' (C', b) N) (NE + UE)) =
         set_mset (all_atms N (NE + UE))\<close> (is ?A)
       \<open>trail_pol (all_atms (fmupd x' (C', b) N) (NE + UE)) =
@@ -2004,13 +2030,13 @@ find_theorems cons_trail_Propagated_tr
         uM_\<L>\<^sub>a\<^sub>l\<^sub>l vdom lcount vdom_m dist_vdom
       apply (subst propagate_bt_wl_D_alt_def)
       unfolding U U' H get_fresh_index_wl_def prod.case
-        propagate_bt_wl_D_heur_alt_def rescore_clause_def hd_tr_S_M
+        propagate_bt_wl_D_heur_alt_def rescore_clause_def
       apply (rewrite in \<open>let _ = _!1 in _\<close> Let_def)
       apply (rewrite in \<open>let _ = update_lbd _ _ _ in _\<close> Let_def)
       apply (rewrite in \<open>let _ = list_update _ (nat_of_lit _) _ in _\<close> Let_def)
       apply (rewrite in \<open>let _ = list_update _ (nat_of_lit _) _ in _\<close> Let_def)
       apply (rewrite in \<open>let _ = False in _\<close> Let_def)
-      apply (refine_rcg cons_trail_Propagated_tr[THEN fref_to_Down_unRET_uncurry2, of \<open>all_atms_st U'\<close>])
+      apply (refine_rcg cons_trail_Propagated_tr2[of _ _ _ _ _ _ \<open>all_atms_st U'\<close>])
       subgoal using valid by (auto dest!: valid_arena_vdom_subset)
       subgoal  using valid size_mset_mono[OF avdom] by (auto dest!: valid_arena_vdom_subset)
       subgoal using \<open>nat_of_lit (C ! Suc 0) < length W'\<close> by simp
@@ -2040,27 +2066,15 @@ find_theorems cons_trail_Propagated_tr
         using M1'_M1
         by (rule cons_trail_Propagated_tr_pre)
           (use undef uM_\<L>\<^sub>a\<^sub>l\<^sub>l in \<open>auto simp: lit_of_hd_trail_def S' U' all_atms_def[symmetric]\<close>)
-      subgoal using undef by (auto simp: S')
-      subgoal using uM_\<L>\<^sub>a\<^sub>l\<^sub>l by (auto simp: S' U' uminus_\<A>\<^sub>i\<^sub>n_iff)
+      subgoal using M1'_M1 by (auto simp: lit_of_hd_trail_def S' U' all_atms_def[symmetric])
+      subgoal using uM_\<L>\<^sub>a\<^sub>l\<^sub>l by (auto simp: S' U' uminus_\<A>\<^sub>i\<^sub>n_iff lit_of_hd_trail_def)
       subgoal
         using D' C_1_neq_hd vmtf avdom
         by (auto simp: propagate_bt_wl_D_heur_def twl_st_heur_def lit_of_hd_trail_st_heur_def
             intro!: ASSERT_refine_left ASSERT_leI RES_refine exI[of _ C] valid_arena_update_lbd
             dest: valid_arena_one_notin_vdomD
             intro!: vm)
-      subgoal
-        using D' C_1_neq_hd vmtf avdom M1'_M1
-        by (auto simp: propagate_bt_wl_D_heur_def twl_st_heur_def lit_of_hd_trail_st_heur_def
-            phase_saving_def atms_of_def S' U' lit_of_hd_trail_def all_atms_def[symmetric])
-      subgoal by auto
-      subgoal
-        using D' C_1_neq_hd vmtf avdom M1'_M1
-        by (auto simp: propagate_bt_wl_D_heur_def twl_st_heur_def lit_of_hd_trail_st_heur_def
-            phase_saving_def atms_of_def S' U' lit_of_hd_trail_def all_atms_def[symmetric])
-      subgoal
-        using D' C_1_neq_hd vmtf avdom M1'_M1
-        by (auto simp: propagate_bt_wl_D_heur_def twl_st_heur_def lit_of_hd_trail_st_heur_def
-            phase_saving_def atms_of_def S' U' lit_of_hd_trail_def all_atms_def[symmetric])
+      apply assumption
       subgoal
         using D' C_1_neq_hd vmtf avdom M1'_M1
         by (auto simp: propagate_bt_wl_D_heur_def twl_st_heur_def lit_of_hd_trail_st_heur_def
@@ -2074,7 +2088,7 @@ find_theorems cons_trail_Propagated_tr
             list_of_mset2_def vmtf_flush_def RES_RES2_RETURN_RES RES_RETURN_RES \<phi> uminus_\<A>\<^sub>i\<^sub>n_iff
             get_fresh_index_def RES_RETURN_RES2 RES_RES_RETURN_RES2 lit_of_hd_trail_def
             RES_RES_RETURN_RES lbd_empty_def get_LBD_def DECISION_REASON_def
-            all_atms_def[symmetric] cons_trail_Propagated_def
+            all_atms_def[symmetric]
             intro!: ASSERT_refine_left ASSERT_leI RES_refine exI[of _ C] valid_arena_update_lbd
             dest: valid_arena_one_notin_vdomD
             simp del: isasat_input_bounded_def isasat_input_nempty_def)
@@ -2083,22 +2097,21 @@ find_theorems cons_trail_Propagated_tr
       done
   qed
 
-  have propagate_unit_bt_wl_D_int: \<open>propagate_unit_bt_wl_D_int
-       (lit_of_hd_trail_st_heur S) U
+  have propagate_unit_bt_wl_D_int: \<open>propagate_unit_bt_wl_D_int LK U
       \<le> \<Down> ?S
-          (propagate_unit_bt_wl_D
-            (lit_of (hd (get_trail_wl S'))) U')\<close>
+          (propagate_unit_bt_wl LK' U')\<close>
     if
       SS': \<open>(S, S') \<in> ?R\<close> and
-      \<open>backtrack_wl_D_inv S'\<close> and
+      \<open>backtrack_wl_inv S'\<close> and
       \<open>backtrack_wl_D_heur_inv S\<close> and
       \<open>(TnC, T') \<in> ?shorter S' S\<close> and
       [simp]: \<open>nC = (n, C)\<close> and
       [simp]: \<open>TnC = (T, nC)\<close> and
       find_decomp: \<open>(U, U') \<in> ?find_decomp S T' n\<close> and
       \<open>\<not> 1 < length C\<close> and
-      \<open>\<not> 1 < size (the (get_conflict_wl U'))\<close>
-    for S S' TnC T' T nC n C U U'
+      \<open>\<not> 1 < size (the (get_conflict_wl U'))\<close> and
+      KK': \<open>(LK, LK') \<in> {(L, L'). L = L' \<and> L = lit_of (hd (get_trail_wl S'))}\<close>
+    for S S' TnC T' T nC n C U U' LK LK'
   proof -
     have
       TT': \<open>(T, del_conflict_wl T') \<in> twl_st_heur_bt\<close> and
@@ -2144,10 +2157,14 @@ find_theorems cons_trail_Propagated_tr
       using \<open>(TnC, T') \<in> ?shorter S' S\<close> find_decomp
       apply (cases U')
       by (auto simp: find_lit_of_max_level_wl_def T')
-    obtain vm' W' \<phi> clvls cach lbd outl stats fema sema ccount vdom avdom lcount arena D' Q' opts
+    have [simp]:
+       \<open>LK' = lit_of (hd (get_trail_wl T'))\<close>
+       \<open>LK = LK'\<close>
+       using KK' SS' S' by (auto simp: T')
+    obtain vm' W' \<phi> clvls cach lbd outl stats heur vdom avdom lcount arena D' Q' opts
       M1'
       where
-        U: \<open>U = (M1', arena, D', Q', W', vm', \<phi>, clvls, cach, lbd, outl, stats, fema, sema, ccount,
+        U: \<open>U = (M1', arena, D', Q', W', vm', \<phi>, clvls, cach, lbd, outl, stats, heur,
            vdom, avdom, lcount, opts, [])\<close> and
         avdom: \<open>mset avdom \<subseteq># mset vdom\<close> and
         r': \<open>length (get_clauses_wl_heur U) = r\<close>
@@ -2179,17 +2196,21 @@ find_theorems cons_trail_Propagated_tr
     have C: \<open>C = [- lit_of (hd M)]\<close>
       using \<open>C \<noteq> []\<close> \<open>C ! 0 = - lit_of (hd M)\<close> \<open>\<not>1 < length C\<close>
       by (cases C) (auto simp del: \<open>C ! 0 = - lit_of (hd M)\<close>)
-    have propagate_unit_bt_wl_D_alt_def:
-      \<open>propagate_unit_bt_wl_D = (\<lambda>L (M, N, D, NE, UE, Q, W). do {
+    have propagate_unit_bt_wl_alt_def:
+      \<open>propagate_unit_bt_wl = (\<lambda>L (M, N, D, NE, UE, Q, W). do {
+        ASSERT(L \<in># all_lits_of_mm (mset `# ran_mf N + (NE + UE)));
+        ASSERT(propagate_unit_bt_wl_pre L (M, N, D, NE, UE, Q, W));
 	_ \<leftarrow> RETURN ();
 	_ \<leftarrow> RETURN ();
 	_ \<leftarrow> RETURN ();
 	_ \<leftarrow> RETURN ();
-	M \<leftarrow> RETURN (cons_trail_Propagated (-L) 0 M);
-        D' \<leftarrow> single_of_mset (the D);
-        RETURN (M, N, None, NE, add_mset {#D'#} UE, {#L#}, W)
+	M \<leftarrow> cons_trail_propagate_l (-L) 0 M;
+        RETURN (M, N, None, NE, add_mset (the D) UE, {#L#}, W)
       })\<close>
-      unfolding propagate_unit_bt_wl_D_def Let_def cons_trail_Propagated_def by auto
+      unfolding propagate_unit_bt_wl_def Let_def by (auto intro!: ext bind_cong[OF refl]
+       simp: propagate_unit_bt_wl_pre_def propagate_unit_bt_l_pre_def
+         single_of_mset_def RES_RETURN_RES image_iff)
+
     have [refine0]:
       \<open>lbd_empty lbd \<le> SPEC (\<lambda>c. (c, ()) \<in> {(c, _). c = replicate (length lbd) False})\<close>
       by (auto simp: lbd_empty_def)
@@ -2226,13 +2247,6 @@ find_theorems cons_trail_Propagated_tr
       unfolding lit_of_hd_trail_def lit_of_hd_trail_st_heur_def
       by (subst lit_of_last_trail_pol_lit_of_last_trail[THEN fref_to_Down_unRET_Id])
         (use M'M tr_S tr_nempty in \<open>auto simp: lit_of_hd_trail_def T' S'\<close>)
-    have [of _ _ \<open>all_atms_st U'\<close>, refine0]: \<open>undefined_lit M L \<and> L \<in># \<L>\<^sub>a\<^sub>l\<^sub>l \<A> \<and> C \<noteq> DECISION_REASON \<Longrightarrow>
-       (((L', C'), M'), (L, C), M) \<in> nat_lit_lit_rel \<times>\<^sub>f nat_rel \<times>\<^sub>f trail_pol \<A> \<Longrightarrow>
-       RETURN (cons_trail_Propagated_tr L' C' M')
-         \<le> \<Down> {(M0, M0''). (M0, M0'') \<in> trail_pol \<A> \<and> M0'' = Propagated L C' # M}
-	     (RETURN (cons_trail_Propagated L C M))\<close> for C C' :: nat and L and L' and M M' \<A>
-      using cons_trail_Propagated_tr[of \<A>, THEN fref_to_Down_curry2, of L C M L' C' M']
-      by (auto simp: cons_trail_Propagated_def)
     have uL_M: \<open>- lit_of (hd (get_trail_wl S')) \<in># \<L>\<^sub>a\<^sub>l\<^sub>l (all_atms_st U')\<close>
       using uL_M by (simp add: S' U')
     let ?NE = \<open>add_mset {#- lit_of (hd M)#} (NE + UE)\<close>
@@ -2306,87 +2320,91 @@ find_theorems cons_trail_Propagated_tr
         done
     qed
 
-    have hd_tr_S_M: \<open>lit_of_hd_trail_st_heur S = lit_of_hd_trail M\<close>
-      unfolding lit_of_hd_trail_def lit_of_hd_trail_st_heur_def
-      by (subst lit_of_last_trail_pol_lit_of_last_trail[THEN fref_to_Down_unRET_Id, OF _ tr_S])
-        (use tr_nempty in \<open>auto simp: lit_of_hd_trail_def T'\<close>)
-
     show ?thesis
       using empty_cach n_d_M1 W'W outl vmtf C \<phi> undef uL_M vdom lcount valid D' avdom
       unfolding U U' propagate_unit_bt_wl_D_int_def prod.simps hd_SM
-        propagate_unit_bt_wl_D_alt_def
+        propagate_unit_bt_wl_alt_def
       apply (rewrite at \<open>let _ = incr_uset _ in _\<close> Let_def)
-      apply (refine_rcg)
+      apply (refine_rcg cons_trail_Propagated_tr2[where \<A> = \<open>all_atms_st U'\<close>])
       subgoal using M'M by (rule isa_length_trail_pre)
       subgoal by (auto simp: DECISION_REASON_def)
       subgoal
         using M'M by (rule cons_trail_Propagated_tr_pre)
-          (use undef uL_M in \<open>auto simp: hd_SM all_atms_def[symmetric] hd_tr_S_M
-	  lit_of_hd_trail_def S'\<close>)
-	    subgoal
-	      by (auto simp: U U' lit_of_hd_trail_st_heur_def RETURN_def
-	          single_of_mset_def vmtf_flush_def twl_st_heur_def lbd_empty_def get_LBD_def
-	          RES_RES2_RETURN_RES RES_RETURN_RES S' uminus_\<A>\<^sub>i\<^sub>n_iff RES_RES_RETURN_RES
-	          DECISION_REASON_def hd_SM
-	          intro!: ASSERT_refine_left RES_refine exI[of _ \<open>-lit_of (hd M)\<close>]
-	          intro!: vmtf_consD
-	          simp del: isasat_input_bounded_def isasat_input_nempty_def)
-	    subgoal
-	      by (auto simp: U U' lit_of_hd_trail_st_heur_def RETURN_def
-	          single_of_mset_def vmtf_flush_def twl_st_heur_def lbd_empty_def get_LBD_def
-	          RES_RES2_RETURN_RES RES_RETURN_RES S' uminus_\<A>\<^sub>i\<^sub>n_iff RES_RES_RETURN_RES
-	          DECISION_REASON_def hd_SM
-	          intro!: ASSERT_refine_left RES_refine exI[of _ \<open>-lit_of (hd M)\<close>]
-	          intro!: vmtf_consD
-	          simp del: isasat_input_bounded_def isasat_input_nempty_def)
-	    subgoal
-	      using M'M
-	      by (auto simp: U U' lit_of_hd_trail_st_heur_def RETURN_def
-	          single_of_mset_def vmtf_flush_def twl_st_heur_def lbd_empty_def get_LBD_def
-	          RES_RES2_RETURN_RES RES_RETURN_RES S' uminus_\<A>\<^sub>i\<^sub>n_iff RES_RES_RETURN_RES
-	          DECISION_REASON_def hd_SM
-	          intro!: ASSERT_refine_left RES_refine exI[of _ \<open>-lit_of (hd M)\<close>]
-	          intro!: vmtf_consD
-	          simp del: isasat_input_bounded_def isasat_input_nempty_def)
-	    subgoal
-	      using bounded nempty dist_vdom r'
-	      by (auto simp: U U' lit_of_hd_trail_st_heur_def RETURN_def
-	          single_of_mset_def vmtf_flush_def twl_st_heur_def lbd_empty_def get_LBD_def
-	          RES_RES2_RETURN_RES RES_RETURN_RES S' uminus_\<A>\<^sub>i\<^sub>n_iff RES_RES_RETURN_RES
-	          DECISION_REASON_def hd_SM All_atms_rew all_atms_def[symmetric]
-	          intro!: ASSERT_refine_left RES_refine exI[of _ \<open>-lit_of (hd M)\<close>]
-	          intro!: isa_vmtf_consD
-	          simp del: isasat_input_bounded_def isasat_input_nempty_def)
-	    done
+           (use undef uL_M in \<open>auto simp: hd_SM all_atms_def[symmetric] T'
+	    lit_of_hd_trail_def S'\<close>)
+     subgoal
+       using M'M by (auto simp: U U' lit_of_hd_trail_st_heur_def RETURN_def
+           single_of_mset_def vmtf_flush_def twl_st_heur_def lbd_empty_def get_LBD_def
+           RES_RES2_RETURN_RES RES_RETURN_RES S' uminus_\<A>\<^sub>i\<^sub>n_iff RES_RES_RETURN_RES
+           DECISION_REASON_def hd_SM lit_of_hd_trail_st_heur_def
+           intro!: ASSERT_refine_left RES_refine exI[of _ \<open>-lit_of (hd M)\<close>]
+           intro!: vmtf_consD
+           simp del: isasat_input_bounded_def isasat_input_nempty_def)
+     subgoal
+       by (auto simp: U U' lit_of_hd_trail_st_heur_def RETURN_def
+           single_of_mset_def vmtf_flush_def twl_st_heur_def lbd_empty_def get_LBD_def
+           RES_RES2_RETURN_RES RES_RETURN_RES S' uminus_\<A>\<^sub>i\<^sub>n_iff RES_RES_RETURN_RES
+           DECISION_REASON_def hd_SM T'
+           intro!: ASSERT_refine_left RES_refine exI[of _ \<open>-lit_of (hd M)\<close>]
+           intro!: vmtf_consD
+           simp del: isasat_input_bounded_def isasat_input_nempty_def)
+     subgoal
+       using bounded nempty dist_vdom r'
+       by (auto simp: U U' lit_of_hd_trail_st_heur_def RETURN_def
+           single_of_mset_def vmtf_flush_def twl_st_heur_def lbd_empty_def get_LBD_def
+           RES_RES2_RETURN_RES RES_RETURN_RES S' uminus_\<A>\<^sub>i\<^sub>n_iff RES_RES_RETURN_RES
+           DECISION_REASON_def hd_SM All_atms_rew all_atms_def[symmetric]
+           intro!: ASSERT_refine_left RES_refine exI[of _ \<open>-lit_of (hd M)\<close>]
+           intro!: isa_vmtf_consD2
+           simp del: isasat_input_bounded_def isasat_input_nempty_def)
+       done
   qed
 
   have trail_nempty: \<open>fst (get_trail_wl_heur S) \<noteq> []\<close>
     if
       \<open>(S, S') \<in> ?R\<close> and
-      \<open>backtrack_wl_D_inv S'\<close>
+      \<open>backtrack_wl_inv S'\<close>
     for S S'
   proof -
     show ?thesis
-      using that unfolding backtrack_wl_D_inv_def backtrack_wl_D_heur_inv_def backtrack_wl_inv_def
+      using that unfolding backtrack_wl_inv_def backtrack_wl_D_heur_inv_def backtrack_l_inv_def backtrack_inv_def
         backtrack_l_inv_def apply -
       by normalize_goal+
         (auto simp:  twl_st_heur_conflict_ana_def trail_pol_def ann_lits_split_reasons_def)
   qed
 
+
+  have [refine]: \<open>\<And>x y. (x, y)
+          \<in> {(S, T).
+             (S, T) \<in> twl_st_heur_conflict_ana \<and>
+             length (get_clauses_wl_heur S) = r} \<Longrightarrow>
+          lit_of_hd_trail_st_heur x
+          \<le> \<Down> {(L, L'). L = L' \<and> L = lit_of (hd (get_trail_wl y))} (mop_lit_hd_trail_wl y)\<close>
+    unfolding mop_lit_hd_trail_wl_def lit_of_hd_trail_st_heur_def
+    apply refine_rcg
+    subgoal unfolding mop_lit_hd_trail_wl_pre_def mop_lit_hd_trail_l_pre_def mop_lit_hd_trail_pre_def
+     by (auto simp:  twl_st_heur_conflict_ana_def mop_lit_hd_trail_wl_pre_def mop_lit_hd_trail_l_pre_def trail_pol_alt_def
+           mop_lit_hd_trail_pre_def state_wl_l_def twl_st_l_def lit_of_hd_trail_def RETURN_RES_refine_iff)
+    subgoal for  x y
+      apply simp_all
+      by (subst lit_of_last_trail_pol_lit_of_last_trail[THEN fref_to_Down_unRET_Id, of \<open>get_trail_wl y\<close> \<open>get_trail_wl_heur x\<close> \<open>all_atms_st y\<close>])
+        (auto simp:  twl_st_heur_conflict_ana_def mop_lit_hd_trail_wl_pre_def mop_lit_hd_trail_l_pre_def
+           mop_lit_hd_trail_pre_def state_wl_l_def twl_st_l_def lit_of_hd_trail_def RETURN_RES_refine_iff)
+    done
   show ?thesis
     supply [[goals_limit=1]]
     apply (intro frefI nres_relI)
-    unfolding backtrack_wl_D_nlit_heur_alt_def backtrack_wl_D_def
+    unfolding backtrack_wl_D_nlit_heur_alt_def backtrack_wl_def
     apply (refine_rcg shorter)
     subgoal by (rule inv)
     subgoal by (rule trail_nempty)
     subgoal for x y xa S x1 x2 x1a x2a
       by (auto simp: twl_st_heur_state_simp equality_except_conflict_wl_get_clauses_wl)
-    apply (rule find_decomp_wl_nlit; solves assumption)
+    apply (rule find_decomp_wl_nlit; assumption)
     subgoal by (auto simp: twl_st_heur_state_simp equality_except_conflict_wl_get_clauses_wl
           equality_except_trail_wl_get_clauses_wl)
-    subgoal for x y xa S x1 x2 x1a x2a Sa Sb
-      by (cases Sb; cases S) (auto simp: twl_st_heur_state_simp)
+    subgoal for x y L La xa S x1 x2 x1a x2a Sa Sb
+      by (auto simp: twl_st_heur_state_simp equality_except_trail_wl_get_conflict_wl)
     apply (rule fst_find_lit_of_max_level_wl; solves assumption)
     apply (rule propagate_bt_wl_D_heur; assumption)
     apply (rule propagate_unit_bt_wl_D_int; assumption)
@@ -2401,8 +2419,8 @@ lemma le_uint32_max_div_2_le_uint32_max: \<open>a \<le> uint32_max div 2 + 1 \<L
 
 
 lemma propagate_bt_wl_D_heur_alt_def:
-  \<open>propagate_bt_wl_D_heur = (\<lambda>L C (M, N0, D, Q, W0, vm0, \<phi>0, y, cach, lbd, outl, stats, fema, sema,
-         res_info, vdom, avdom, lcount, opts). do {
+  \<open>propagate_bt_wl_D_heur = (\<lambda>L C (M, N0, D, Q, W0, vm0, \<phi>0, y, cach, lbd, outl, stats, (fema, sema,
+         res_info), vdom, avdom, lcount, opts). do {
       ASSERT(length vdom \<le> length N0);
       ASSERT(length avdom \<le> length N0);
       ASSERT(nat_of_lit (C!1) < length W0 \<and> nat_of_lit (-L) < length W0);
@@ -2413,30 +2431,30 @@ lemma propagate_bt_wl_D_heur_alt_def:
       glue \<leftarrow> get_LBD lbd;
       let b = False;
       let b' = (length C = 2);
-      ASSERT(isasat_fast (M, N0, D, Q, W0, vm0, \<phi>0, y, cach, lbd, outl, stats, fema, sema,
-         res_info, vdom, avdom, lcount, opts) \<longrightarrow> append_and_length_fast_code_pre ((b, C), N0));
-      ASSERT(isasat_fast (M, N0, D, Q, W0, vm0, \<phi>0, y, cach, lbd, outl, stats, fema, sema,
-         res_info, vdom, avdom, lcount, opts) \<longrightarrow> lcount < sint64_max);
+      ASSERT(isasat_fast (M, N0, D, Q, W0, vm0, \<phi>0, y, cach, lbd, outl, stats, (fema, sema,
+         res_info), vdom, avdom, lcount, opts) \<longrightarrow> append_and_length_fast_code_pre ((b, C), N0));
+      ASSERT(isasat_fast (M, N0, D, Q, W0, vm0, \<phi>0, y, cach, lbd, outl, stats, (fema, sema,
+         res_info), vdom, avdom, lcount, opts) \<longrightarrow> lcount < sint64_max);
       (N, i) \<leftarrow> fm_add_new_fast b C N0;
       ASSERT(update_lbd_pre ((i, glue), N));
       let N = update_lbd i glue N;
-      ASSERT(isasat_fast (M, N0, D, Q, W0, vm0, \<phi>0, y, cach, lbd, outl, stats, fema, sema,
-         res_info, vdom, avdom, lcount, opts) \<longrightarrow> length_ll W0 (nat_of_lit (-L)) < sint64_max);
+      ASSERT(isasat_fast (M, N0, D, Q, W0, vm0, \<phi>0, y, cach, lbd, outl, stats, (fema, sema,
+         res_info), vdom, avdom, lcount, opts) \<longrightarrow> length_ll W0 (nat_of_lit (-L)) < sint64_max);
       let W = W0[nat_of_lit (- L) := W0 ! nat_of_lit (- L) @ [(i, L', b')]];
-      ASSERT(isasat_fast (M, N0, D, Q, W0, vm0, \<phi>0, y, cach, lbd, outl, stats, fema, sema,
-         res_info, vdom, avdom, lcount, opts) \<longrightarrow> length_ll W (nat_of_lit L') < sint64_max);
+      ASSERT(isasat_fast (M, N0, D, Q, W0, vm0, \<phi>0, y, cach, lbd, outl, stats, (fema, sema,
+         res_info), vdom, avdom, lcount, opts) \<longrightarrow> length_ll W (nat_of_lit L') < sint64_max);
       let W = W[nat_of_lit L' := W!nat_of_lit L' @ [(i, -L, b')]];
       lbd \<leftarrow> lbd_empty lbd;
       ASSERT(isa_length_trail_pre M);
       let j = isa_length_trail M;
       ASSERT(i \<noteq> DECISION_REASON);
       ASSERT(cons_trail_Propagated_tr_pre ((-L, i), M));
-      let M = cons_trail_Propagated_tr (- L) i M;
+      M \<leftarrow> cons_trail_Propagated_tr (- L) i M;
       vm \<leftarrow> isa_vmtf_flush_int M vm;
       ASSERT(atm_of L < length \<phi>);
       RETURN (M, N, D, j, W, vm, save_phase (-L) \<phi>, 0,
-         cach, lbd, outl, add_lbd (of_nat glue) stats, ema_update glue fema, ema_update glue sema,
-          incr_conflict_count_since_last_restart res_info, vdom @ [i],
+         cach, lbd, outl, add_lbd (of_nat glue) stats, (ema_update glue fema, ema_update glue sema,
+          incr_conflict_count_since_last_restart res_info), vdom @ [i],
           avdom @ [i],
           lcount + 1, opts)
     })\<close>
@@ -2456,7 +2474,7 @@ lemma propagate_bt_wl_D_fast_code_isasat_fastI3: \<open>isasat_fast b \<Longrigh
   by (cases b) (auto simp: isasat_fast_def sint64_max_def uint32_max_def)
 
 lemma lit_of_hd_trail_st_heur_alt_def:
-  \<open>lit_of_hd_trail_st_heur = (\<lambda>(M, N, D, Q, W, vm, \<phi>). lit_of_last_trail_pol M)\<close>
+  \<open>lit_of_hd_trail_st_heur = (\<lambda>(M, N, D, Q, W, vm, \<phi>). do {ASSERT (fst M \<noteq> []); RETURN (lit_of_last_trail_pol M)})\<close>
   by (auto simp: lit_of_hd_trail_st_heur_def lit_of_hd_trail_def intro!: ext)
 
 end
