Weidenbach_Book/IsaSAT_Inner_Propagation_LLVM.thy
@@ -296,10 +296,6 @@ export_llvm
   set_conflict_wl_heur_fast_code
   unit_propagation_inner_loop_body_wl_fast_heur_code
 
-
 end
-
-
-
 
 end
