Weidenbach_Book/IsaSAT_Propagate_Conflict_LLVM.thy
@@ -177,8 +177,6 @@ export_llvm
   select_and_remove_from_literals_to_update_wlfast_code
   literals_to_update_wl_literals_to_update_wl_empty_fast_code
   unit_propagation_outer_loop_wl_D_fast_code
- 
-
 
 end
 
